better SequenceEqual

StandardLibrary/src/Sequence.dfy
@@ -1,28 +1,41 @@
 // Copyright Amazon.com Inc. or its affiliates. All Rights Reserved.
 // SPDX-License-Identifier: Apache-2.0
 
+include "UInt.dfy"
+
 module StandardLibrary.Sequence {
-  export provides SequenceEqual
+  // export provides SequenceEqual, StandardLibrary
+  import opened UInt
 
-  /* No Allocation Comparison of two Sequences. Author: ajewellamz */
-  predicate method SequenceEqual<T(==)>(
-    nameonly seq1 : seq<T>,
-    nameonly seq2 : seq<T>,
-    nameonly start1 : nat,
-    nameonly start2 : nat,
-    nameonly size : nat
-  ): (ret: bool) // returns (ret : bool)
+predicate method SequenceEqualNat<T(==)>(seq1: seq<T>, seq2: seq<T>, start1: nat, start2: nat, size: nat) : (ret : bool)
+  requires start1 + size <= |seq1|
+  requires start2 + size <= |seq2|
+  ensures ret ==> seq1[start1..start1 + size] == seq2[start2..start2 + size]
+{
+  if |seq1| > INT64_MAX_LIMIT || |seq2| > INT64_MAX_LIMIT then
+    false
+  else
+    SequenceEqual(seq1, seq2, start1 as uint64, start2 as uint64, size as uint64)
+}
 
-    requires start1 + size <= |seq1|
-    requires start2 + size <= |seq2|
-    ensures ret ==> seq1[start1 .. start1 + size] == seq2[start2 .. start2+size]
+predicate SequenceEqual<T(==)>(seq1: seq64<T>, seq2: seq64<T>, start1: uint64, start2: uint64, size: uint64) : (ret : bool)
+  requires start1 as nat + size as nat <= |seq1| 
+  requires start2 as nat + size as nat <= |seq2|
+  ensures ret <==> seq1[start1..start1 + size] == seq2[start2..start2 + size]
+{
+  seq1[start1..start1 + size] == seq2[start2..start2 + size]
+} by method {
+  var j := start2 as uint64;
+  for i := start1 as uint64 to (start1 + size) as uint64
+    invariant j == i - start1 + start2
+    invariant forall k : uint64 | start1 <= k < i :: seq1[k] == seq2[k - start1 + start2]
   {
-    // for i : nat := 0 to size {
-    //   if seq1[start1+i] != seq2[start2+i] {
-    //     return false;
-    //   }
-    // }
-    // return true;
-    forall i | 0 <= i < size :: seq1[start1+i] == seq2[start2+i]
+    if seq1[i] != seq2[j] {
+      return false;
+    }
+    j := j + 1;
   }
+  return true;
+}
+
 }
